Sums: no longer use dependent pairs

src/lowparse/LowParse.Spec.Sum.fst
@@ -4,76 +4,83 @@ include LowParse.Spec.Enum
 module Seq = FStar.Seq
 
 inline_for_extraction
+let refine_with_tag (#tag_t: Type0) (#data_t: Type0) (tag_of_data: (data_t -> GTot tag_t)) (x: tag_t) : Tot Type0 =
+  (y: data_t { tag_of_data y == x } )
+
 val parse_tagged_union
   (#kt: parser_kind)
-  (#tag: Type0)
-  (#tu: tag -> Type0)
-  (pt: parser kt tag)
+  (#tag_t: Type0)
+  (pt: parser kt tag_t)
+  (#data_t: Type0)
+  (tag_of_data: (data_t -> GTot tag_t))
   (#k: parser_kind)
-  (p: (t: tag) -> Tot (parser k (tu t))) // Tot really needed here by validator
-: Tot (parser (and_then_kind kt k) (t: tag & tu t))
+  (p: (t: tag_t) -> Tot (parser k (refine_with_tag tag_of_data t)))
+: Tot (parser (and_then_kind kt k) data_t)
 
-let parse_tagged_union #kt #tag #tu pt #k p =
-  pt `and_then` (fun (v: tag) ->
-    let pv : parser k (tu v) = p v in
-    let synth : tu v -> Tot (t: tag & tu t) = fun (v': tu v) -> (| v, v' |) in
-    parse_synth #k #(tu v) #(t: tag & tu t) pv synth
+let parse_tagged_union #kt #tag_t pt #data_t tag_of_data #k p =
+  pt `and_then` (fun (tg: tag_t) ->
+    let ptg : parser k (refine_with_tag tag_of_data tg) = p tg in
+    let synth : refine_with_tag tag_of_data tg -> Tot data_t = fun x -> x in
+    parse_synth #k #(refine_with_tag tag_of_data tg) ptg synth
   )
 
 let bare_serialize_tagged_union
   (#kt: parser_kind)
-  (#tag: Type0)
-  (#tu: tag -> Type0)
-  (pt: parser kt tag)
+  (#tag_t: Type0)
+  (#pt: parser kt tag_t)
   (st: serializer pt)
+  (#data_t: Type0)
+  (tag_of_data: (data_t -> GTot tag_t))
   (#k: parser_kind)
-  (p: (t: tag) -> Tot (parser k (tu t))) // Tot really needed here by validator
-  (s: (t: tag) -> Tot (serializer (p t)))
-: Tot (bare_serializer (t: tag & tu t))
-= fun (x: (t: tag & tu t)) ->
-  let (| t, u |) = x in
-  Seq.append (st t) (serialize (s t) u)
+  (#p: (t: tag_t) -> Tot (parser k (refine_with_tag tag_of_data t)))
+  (s: (t: tag_t) -> Tot (serializer (p t)))
+: Tot (bare_serializer data_t)
+= fun (d: data_t) ->
+  let tg = tag_of_data d in
+  Seq.append (st tg) (serialize (s tg) d)
 
 #set-options "--z3rlimit 16"
 
 let bare_serialize_tagged_union_correct
   (#kt: parser_kind)
-  (#tag: Type0)
-  (#tu: tag -> Type0)
-  (pt: parser kt tag)
+  (#tag_t: Type0)
+  (#pt: parser kt tag_t)
   (st: serializer pt)
+  (#data_t: Type0)
+  (tag_of_data: (data_t -> GTot tag_t))
   (#k: parser_kind)
-  (p: (t: tag) -> Tot (parser k (tu t))) // Tot really needed here by validator
-  (s: (t: tag) -> Tot (serializer (p t)))
+  (#p: (t: tag_t) -> Tot (parser k (refine_with_tag tag_of_data t)))
+  (s: (t: tag_t) -> Tot (serializer (p t)))
 : Lemma
   (requires (kt.parser_kind_subkind == Some ParserStrong))
-  (ensures (serializer_correct (parse_tagged_union pt p) (bare_serialize_tagged_union pt st p s)))
+  (ensures (serializer_correct (parse_tagged_union pt tag_of_data p) (bare_serialize_tagged_union st tag_of_data s)))
 = (* same proof as nondep_then *)
   let prf
-    (x: (t: tag & tu t))
-  : Lemma (parse (parse_tagged_union pt p) (bare_serialize_tagged_union pt st p s x) == Some (x, Seq.length (bare_serialize_tagged_union pt st p s x)))
-  = let (| t, u |) = x in
-    let v1' = parse pt (bare_serialize_tagged_union pt st p s x) in
+    (x: data_t)
+  : Lemma (parse (parse_tagged_union pt tag_of_data p) (bare_serialize_tagged_union st tag_of_data s x) == Some (x, Seq.length (bare_serialize_tagged_union  st tag_of_data s x)))
+  = let t = tag_of_data x in
+    let (u: refine_with_tag tag_of_data t) = x in
+    let v1' = parse pt (bare_serialize_tagged_union st tag_of_data s x) in
     let v1 = parse pt (st t) in
     assert (Some? v1);
-    assert (no_lookahead_on pt (st t) (bare_serialize_tagged_union pt st p s x));
+    assert (no_lookahead_on pt (st t) (bare_serialize_tagged_union st tag_of_data s x));
     let (Some (_, len')) = parse pt (st t) in
     assert (len' == Seq.length (st t));
-    assert (len' <= Seq.length (bare_serialize_tagged_union pt st p s x));
+    assert (len' <= Seq.length (bare_serialize_tagged_union st tag_of_data s x));
     assert (Seq.slice (st t) 0 len' == st t);
     seq_slice_append_l (st t) (serialize (s t) u);
-    assert (no_lookahead_on_precond pt (st t) (bare_serialize_tagged_union pt st p s x));
-    assert (no_lookahead_on_postcond pt (st t) (bare_serialize_tagged_union pt st p s x));
+    assert (no_lookahead_on_precond pt (st t) (bare_serialize_tagged_union st tag_of_data s x));
+    assert (no_lookahead_on_postcond pt (st t) (bare_serialize_tagged_union st tag_of_data s x));
     assert (Some? v1');
-    assert (injective_precond pt (st t) (bare_serialize_tagged_union pt st p s x));
-    assert (injective_postcond pt (st t) (bare_serialize_tagged_union pt st p s x));
+    assert (injective_precond pt (st t) (bare_serialize_tagged_union st tag_of_data s x));
+    assert (injective_postcond pt (st t) (bare_serialize_tagged_union st tag_of_data s x));
     let (Some (x1, len1)) = v1 in
     let (Some (x1', len1')) = v1' in
     assert (x1 == x1');
     assert ((len1 <: nat) == (len1' <: nat));
     assert (x1 == t);
     assert (len1 == Seq.length (st t));
-    assert (bare_serialize_tagged_union pt st p s x == Seq.append (st t) (serialize (s t) u));
+    assert (bare_serialize_tagged_union st tag_of_data s x == Seq.append (st t) (serialize (s t) u));
     seq_slice_append_r (st t) (serialize (s t) u);
     ()
   in
@@ -83,22 +90,23 @@ let bare_serialize_tagged_union_correct
 
 let serialize_tagged_union
   (#kt: parser_kind)
-  (#tag: Type0)
-  (#tu: tag -> Type0)
-  (pt: parser kt tag)
+  (#tag_t: Type0)
+  (#pt: parser kt tag_t)
   (st: serializer pt)
+  (#data_t: Type0)
+  (tag_of_data: (data_t -> GTot tag_t))
   (#k: parser_kind)
-  (p: (t: tag) -> Tot (parser k (tu t))) // Tot really needed here by validator
-  (s: (t: tag) -> Tot (serializer (p t)))
-: Pure (serializer (parse_tagged_union pt p))
+  (#p: (t: tag_t) -> Tot (parser k (refine_with_tag tag_of_data t)))
+  (s: (t: tag_t) -> Tot (serializer (p t)))
+: Pure (serializer (parse_tagged_union pt tag_of_data p))
   (requires (kt.parser_kind_subkind == Some ParserStrong))
   (ensures (fun _ -> True))
-= bare_serialize_tagged_union_correct pt st p s;
-  bare_serialize_tagged_union pt st p s
+= bare_serialize_tagged_union_correct st tag_of_data s;
+  bare_serialize_tagged_union st tag_of_data s
 
 
 inline_for_extraction
-let sum = (key: eqtype & (repr: eqtype & (e: enum key repr & ((x: enum_key e) -> Tot Type0))))
+let sum = (key: eqtype & (repr: eqtype & (e: enum key repr & ((data: Type0) & (tag_of_data: (data -> GTot (enum_key e)))))))
 
 inline_for_extraction
 let sum_key_type (t: sum) : Tot eqtype =
@@ -108,17 +116,28 @@ inline_for_extraction
 let sum_repr_type (t: sum) : Tot eqtype =
   let (| _, (| repr,  _ |) |) = t in repr
 
+inline_for_extraction
 let sum_enum (t: sum) : Tot (enum (sum_key_type t) (sum_repr_type t)) =
   let (| _, (| _, (| e, _ |) |) |) = t in e
 
+inline_for_extraction
 let sum_key (t: sum) : Tot Type0 =
   enum_key (sum_enum t)
 
+inline_for_extraction
 let sum_cases (t: sum) : Tot ((x: sum_key t) -> Tot Type0) =
-  let (|_, (| _, (| _, c |) |) |) = t in c
+  let (|_, (| _, (| _, (| _, tag_of_data |) |) |) |) = t in
+  (fun x -> refine_with_tag tag_of_data x)
 
+inline_for_extraction
 let sum_type (t: sum) : Tot Type0 =
-  (x: sum_key t & sum_cases t x)
+  let (|_, (| _, (| _, (| data, _ |) |) |) |) = t in
+  data
+
+inline_for_extraction
+let sum_tag_of_data (t: sum) : Tot ((x: sum_type t) -> GTot (sum_key t)) =
+  let (|_, (| _, (| _, (| _, tag_of_data |) |) |) |) = t in
+  tag_of_data
 
 let weaken_parse_cases_kind
   (s: sum)
@@ -139,7 +158,6 @@ let parse_sum_cases
 = let (| _, p |) = f x in
   weaken (weaken_parse_cases_kind s f) p
 
-inline_for_extraction
 let parse_sum
   (#kt: parser_kind)
   (t: sum)
@@ -150,18 +168,19 @@ let parse_sum
 = parse_tagged_union
     #(parse_filter_kind kt)
     #(sum_key t)
-    #(fun (c: sum_key t) -> sum_cases t c) // eta-expansion required here because of the eta-expansion in parse_tagged_union, which could not unify with serialize_sum if not eta-expanded here
     (parse_enum_key p (sum_enum t))
+    #(sum_type t)
+    (sum_tag_of_data t)
     #k
     pc
 
 let serialize_sum
   (#kt: parser_kind)
   (t: sum)
-  (p: parser kt (sum_repr_type t))
+  (#p: parser kt (sum_repr_type t))
   (s: serializer p)
   (#k: parser_kind)
-  (pc: ((x: sum_key t) -> Tot (parser k (sum_cases t x))))
+  (#pc: ((x: sum_key t) -> Tot (parser k (sum_cases t x))))
   (sc: ((x: sum_key t) -> Tot (serializer (pc x))))
 : Pure (serializer (parse_sum t p pc))
   (requires (kt.parser_kind_subkind == Some ParserStrong))
@@ -169,97 +188,174 @@ let serialize_sum
 = serialize_tagged_union
     #(parse_filter_kind kt)
     #(sum_key t)
-    #(sum_cases t)
-    (parse_enum_key p (sum_enum t))
+    #(parse_enum_key p (sum_enum t))
     (serialize_enum_key p s (sum_enum t))
+    #(sum_type t)
+    (sum_tag_of_data t)
     #k
-    pc
+    #pc
     sc
 
 inline_for_extraction
 let make_sum
   (#key #repr: eqtype)
   (e: enum key repr)
-  (cases: (enum_key e -> Tot Type0))
+  (#data: Type0)
+  (tag_of_data: (data -> GTot (enum_key e)))
 : Tot sum
-= (| key, (| repr, (| e, cases |) |) |)
+= (| key, (| repr, (| e, (| data, tag_of_data |) |) |) |)
 
 (* Sum with default case *)
 
 inline_for_extraction
 let dsum = (sum * Type0)
 
-let dsum_key (t: dsum) : Tot Type0 =
-  maybe_enum_key (sum_enum (fst t))
-
-let dsum_cases (t: dsum) (x: dsum_key t): Tot Type0 =
-  match x with
-  | Known x -> sum_cases (fst t) x
-  | Unknown x -> snd t
-
-let dsum_type (t: dsum) : Tot Type0 =
-  (x: dsum_key t & dsum_cases t x)
-
-let parse_dsum_cases
-  (s: dsum)
-  (#k: parser_kind)
-  (pc: ((x: sum_key (fst s)) -> Tot (parser k (sum_cases (fst s) x))))
-  (pd: parser k (snd s))
-  (x: dsum_key s)
-: Tot (parser k (dsum_cases s x))
-= match x with
-  | Known x -> pc x
-  | Unknown _ -> pd
-
-let serialize_dsum_cases
-  (s: dsum)
-  (#k: parser_kind)
-  (pc: ((x: sum_key (fst s)) -> Tot (parser k (sum_cases (fst s) x))))
-  (sc: ((x: sum_key (fst s)) -> Tot (serializer (pc x))))
-  (pd: parser k (snd s))
-  (sd: serializer pd)
-  (x: dsum_key s)
-: Tot (serializer (parse_dsum_cases s pc pd x))
-= match x with
-  | Known x -> sc x
-  | Unknown _ -> sd
+type maybe_data (known_data: Type0) (unknown_repr: eqtype) (unknown_data: Type0) =
+  | KnownData : (d: known_data) -> maybe_data known_data unknown_repr unknown_data
+  | UnknownData : (r: unknown_repr) -> (d: unknown_data) -> maybe_data known_data unknown_repr unknown_data
 
 inline_for_extraction
-let parse_dsum
-  (#kt: parser_kind)
+let sum_of_dsum
+  (d: dsum)
+: Tot sum
+= let (s, _) = d in s
+
+inline_for_extraction
+let dsum_key (t: dsum) : Tot Type0 =
+  maybe_enum_key (sum_enum (sum_of_dsum t))
+
+inline_for_extraction
+let dsum_unknown_type
   (t: dsum)
-  (p: parser kt (sum_repr_type (fst t)))
+: Tot Type0
+= let (_, ud) = t in
+  ud
+
+inline_for_extraction
+let dsum_type
+  (t: dsum)
+: Tot Type0
+= maybe_data
+    (sum_type (sum_of_dsum t)) 
+    (unknown_enum_repr (sum_enum (sum_of_dsum t)))
+    (dsum_unknown_type t)
+
+inline_for_extraction
+let dsum_tag_of_data
+  (d: dsum)
+  (data: dsum_type d)
+: GTot (dsum_key d)
+= match data with
+  | KnownData kd -> Known (sum_tag_of_data (sum_of_dsum d) kd)
+  | UnknownData r _ -> Unknown r
+
+inline_for_extraction
+let synth_dsum_known
+  (d: dsum)
+  (kt: sum_key (sum_of_dsum d))
+  (d' : sum_cases (sum_of_dsum d) kt)
+: Tot (refine_with_tag (dsum_tag_of_data d) (Known kt))
+= (KnownData d' <: dsum_type d)
+
+inline_for_extraction
+let synth_dsum_unknown
+  (d: dsum)
+  (r: unknown_enum_repr (sum_enum (sum_of_dsum d)))
+  (d' : dsum_unknown_type d)
+: Tot (refine_with_tag (dsum_tag_of_data d) (Unknown r))
+= (UnknownData r d' <: dsum_type d)
+
+let parse_dsum_cases
+  (d: dsum)
   (#k: parser_kind)
-  (pc: ((x: sum_key (fst t)) -> Tot (parser k (sum_cases (fst t) x))))
-  (pd: parser k (snd t))
-: Tot (parser (and_then_kind kt k) (dsum_type t))
+  (pk: ((kt: sum_key (sum_of_dsum d)) -> Tot (parser k (sum_cases (sum_of_dsum d) kt))))
+  (pu: parser k (dsum_unknown_type d))
+  (t: dsum_key d)
+: Tot (parser k (refine_with_tag (dsum_tag_of_data d) t))
+= match t with
+  | Known kt ->
+    parse_synth (pk kt) (synth_dsum_known d kt)
+  | Unknown r ->
+    parse_synth pu (synth_dsum_unknown d r)
+
+let parse_dsum
+  (d: dsum)
+  (#tk: parser_kind)
+  (tp: parser tk (sum_repr_type (sum_of_dsum d)))
+  (#k: parser_kind)
+  (pk: ((kt: sum_key (sum_of_dsum d)) -> Tot (parser k (sum_cases (sum_of_dsum d) kt))))
+  (pu: parser k (dsum_unknown_type d))
+: Tot (parser (and_then_kind tk k) (dsum_type d))
 = parse_tagged_union
-    #kt
-    #(dsum_key t)
-    #(fun (c: dsum_key t) -> dsum_cases t c) // same as above
-    (parse_maybe_enum_key p (sum_enum (fst t)))
+    #tk
+    #(dsum_key d)
+    (parse_maybe_enum_key tp (sum_enum (sum_of_dsum d)))
+    #(dsum_type d)
+    (dsum_tag_of_data d)
     #k
-    (parse_dsum_cases t pc pd)
+    (parse_dsum_cases d pk pu)
+
+inline_for_extraction
+let synth_dsum_known_recip
+  (d: dsum)
+  (kt: sum_key (sum_of_dsum d))
+  (d' : refine_with_tag (dsum_tag_of_data d) (Known kt))
+: Tot (sum_cases (sum_of_dsum d) kt)
+= let (KnownData d_) = (d' <: dsum_type d) in d_
+
+inline_for_extraction
+let synth_dsum_unknown_recip
+  (d: dsum)
+  (r: unknown_enum_repr (sum_enum (sum_of_dsum d)))
+  (d' : refine_with_tag (dsum_tag_of_data d) (Unknown r)) 
+: Tot (dsum_unknown_type d)
+= let (UnknownData r d_) = (d' <: dsum_type d) in d_
+
+let serialize_dsum_cases
+  (d: dsum)
+  (#k: parser_kind)
+  (#pk: ((kt: sum_key (sum_of_dsum d)) -> Tot (parser k (sum_cases (sum_of_dsum d) kt))))
+  (sk: ((kt: sum_key (sum_of_dsum d)) -> Tot (serializer (pk kt))))
+  (#pu: parser k (dsum_unknown_type d))
+  (su: serializer pu)
+  (t: dsum_key d)
+: Tot (serializer (parse_dsum_cases d pk pu t))
+= match t with
+  | Known kt ->
+    serialize_synth
+      _
+      (synth_dsum_known d kt)
+      (sk kt)
+      (synth_dsum_known_recip d kt)
+      ()
+  | Unknown r ->
+    serialize_synth
+      _
+      (synth_dsum_unknown d r)
+      su
+      (synth_dsum_unknown_recip d r)
+      ()
 
 let serialize_dsum
-  (#kt: parser_kind)
-  (t: dsum)
-  (p: parser kt (sum_repr_type (fst t)))
-  (s: serializer p)
+  (d: dsum)
+  (#tk: parser_kind)
+  (#tp: parser tk (sum_repr_type (sum_of_dsum d)))
+  (ts: serializer tp)
   (#k: parser_kind)
-  (pc: ((x: sum_key (fst t)) -> Tot (parser k (sum_cases (fst t) x))))
-  (sc: ((x: sum_key (fst t)) -> Tot (serializer (pc x))))
-  (pd: parser k (snd t))
-  (sd: serializer pd)
-: Pure (serializer (parse_dsum t p pc pd))
-  (requires (kt.parser_kind_subkind == Some ParserStrong))
+  (#pk: ((kt: sum_key (sum_of_dsum d)) -> Tot (parser k (sum_cases (sum_of_dsum d) kt))))
+  (sk: ((kt: sum_key (sum_of_dsum d)) -> Tot (serializer (pk kt))))
+  (#pu: parser k (dsum_unknown_type d))
+  (su: serializer pu)
+: Pure (serializer (parse_dsum d tp pk pu))
+  (requires (tk.parser_kind_subkind == Some ParserStrong))
   (ensures (fun _ -> True))
 = serialize_tagged_union
-    #kt
-    #(dsum_key t)
-    #(dsum_cases t)
-    (parse_maybe_enum_key p (sum_enum (fst t)))
-    (serialize_maybe_enum_key p s (sum_enum (fst t)))
+    #tk
+    #(dsum_key d)
+    #(parse_maybe_enum_key tp (sum_enum (sum_of_dsum d)))
+    (serialize_maybe_enum_key _ ts (sum_enum (sum_of_dsum d)))
+    #(dsum_type d)
+    (dsum_tag_of_data d)
     #k
-    (parse_dsum_cases t pc pd)
-    (serialize_dsum_cases t pc sc pd sd)
+    #(parse_dsum_cases d pk pu)
+    (serialize_dsum_cases d sk su)
